pcuic/theories/Conversion/PCUICNamelessConv.v
@@ -3,7 +3,7 @@ From Coq Require Import RelationClasses.
 From MetaCoq.Template Require Import config utils.
 From MetaCoq.PCUIC Require Import PCUICAst PCUICOnOne PCUICAstUtils PCUICInduction PCUICCases
      PCUICLiftSubst PCUICEquality PCUICReduction PCUICCumulativitySpec PCUICCumulativity PCUICPosition PCUICUnivSubst
-     PCUICContextRelation PCUICNamelessDef PCUICGuardCondition PCUICClosedConv PCUICClosedTyp PCUICUnivSubstitutionConv
+     PCUICNamelessDef PCUICGuardCondition PCUICClosedConv PCUICClosedTyp PCUICUnivSubstitutionConv
      PCUICClosed PCUICSigmaCalculus (* for context manipulations *).
 Require Import Equations.Prop.DepElim.
 Require Import ssreflect.
