pcuic/theories/PCUICConfluence.v
@@ -2,7 +2,7 @@
 From MetaCoq.Template Require Import config utils.
 From MetaCoq.PCUIC Require Import PCUICAst PCUICOnOne PCUICAstUtils PCUICLiftSubst PCUICTyping
      PCUICReduction PCUICEquality PCUICUnivSubstitutionConv
-     PCUICContextRelation PCUICSigmaCalculus PCUICContextReduction PCUICContextRelation
+     PCUICSigmaCalculus PCUICContextReduction PCUICContextRelation
      PCUICParallelReduction PCUICParallelReductionConfluence PCUICClosedConv PCUICClosedTyp
      PCUICRedTypeIrrelevance PCUICOnFreeVars PCUICInstDef PCUICInstConv PCUICWeakeningConv PCUICWeakeningTyp. 
 
