pcuic/theories/PCUICWellScopedCumulativity.v
@@ -3,7 +3,7 @@ From Coq Require Import ssreflect ssrbool.
 From MetaCoq.Template Require Import config utils.
 From MetaCoq.PCUIC Require Import PCUICAst PCUICAstUtils PCUICLiftSubst PCUICTyping PCUICCumulativity
      PCUICReduction PCUICWeakeningConv PCUICWeakeningTyp PCUICEquality PCUICUnivSubstitutionConv
-     PCUICContextRelation PCUICSigmaCalculus PCUICContextReduction PCUICContextRelation
+     PCUICSigmaCalculus PCUICContextReduction PCUICContextRelation
      PCUICParallelReduction PCUICParallelReductionConfluence PCUICClosedConv PCUICClosedTyp
      PCUICRedTypeIrrelevance PCUICOnFreeVars PCUICConfluence PCUICSubstitution.
 
