pcuic/theories/Typing/PCUICRenameTyp.v
@@ -2,7 +2,7 @@
 From Coq Require Import Morphisms.
 From MetaCoq.Template Require Import config utils.
 From MetaCoq.PCUIC Require Import PCUICAst PCUICAstUtils PCUICCases PCUICInduction
-  PCUICLiftSubst PCUICUnivSubst PCUICContextRelation PCUICCumulativity
+  PCUICLiftSubst PCUICUnivSubst PCUICCumulativity
   PCUICTyping PCUICReduction PCUICGlobalEnv PCUICClosed PCUICEquality PCUICRenameDef 
   PCUICSigmaCalculus PCUICClosed PCUICOnFreeVars PCUICOnFreeVarsConv PCUICGuardCondition PCUICTyping
   PCUICWeakeningEnvConv PCUICWeakeningEnvTyp PCUICClosedConv PCUICClosedTyp PCUICRenameConv.
